code/ecdsap256sha2/Hacl.Impl.P256.MM.Exponent.fsti
@@ -30,3 +30,11 @@ open Spec.P256.Lemmas
 open Spec.P256
 open Spec.P256.Ladder
 open Spec.P256.MontgomeryMultiplication
+
+
+val square_root: a: felem -> result: felem ->  Stack unit 
+  (requires fun h -> live h a /\ live h result /\ as_nat h a < prime)
+  (ensures fun h0 _ h1 -> modifies (loc a |+| loc result) h0 h1 /\
+    fromDomain_ (as_nat h1 result) = sq_root_spec (fromDomain_ (as_nat h0 a)) /\
+    fromDomain_ (as_nat h1 result) = pow (fromDomain_ (as_nat h0 a)) ((prime256 + 1) / 4) % prime256
+  )
