code/ecdsap256sha2/Hacl.Impl.P256.Signature.Common.fsti
@@ -12,6 +12,7 @@ open Spec.P256
 open Spec.P256.Definitions
 
 open Spec.ECDSA
+open Spec.P256.Lemmas
 open Spec.ECDSAP256.Definition
 
 open Hacl.Impl.P256
@@ -39,12 +40,6 @@ val toUint64ChangeEndian: i:lbuffer uint8 (size 32) -> o:felem -> Stack unit
     modifies (loc o) h0 h1 /\
     as_seq h1 o == Spec.ECDSA.changeEndian (uints_from_bytes_be (as_seq h0 i))
   )
-
-val lemma_core_0: a:lbuffer uint64 (size 4) -> h:mem
-  -> Lemma (nat_from_intseq_le (as_seq h a) == as_nat h a)
-
-val lemma_core_1: a:lbuffer uint64 (size 4) -> h:mem ->
-  Lemma (nat_from_bytes_le (uints_to_bytes_le (as_seq h a)) == as_nat h a)
 
 val bufferToJac: p:lbuffer uint64 (size 8) -> result:point -> Stack unit
   (requires fun h -> live h p /\ live h result /\ disjoint p result)
